src/Std/Data/TreeSet/Raw.lean
@@ -158,6 +158,20 @@ differently: it will overwrite an existing mapping.
 def insertIfNew (t : Raw α cmp) (a : α) : Raw α cmp :=
     letI : Ord α := ⟨cmp⟩; ⟨t.inner.insertIfNew a ()⟩
 
+/--
+Checks whether an element is present in a set and inserts the element if it was not found.
+If the hash set already contains an element that is equal (with regard to `==`) to the given
+element, then the hash set is returned unchanged.
+
+Equivalent to (but potentially faster than) calling `contains` followed by `insert`.
+-/
+@[inline]
+def containsThenInsertIfNew [BEq α] [Hashable α] (t : Raw α cmp) (a : α) :
+    Bool × Raw α cmp :=
+  letI : Ord α := ⟨cmp⟩
+  let p := t.inner.containsThenInsertIfNew a ()
+  (p.1, ⟨p.2⟩)
+
 instance : Membership α (Raw α cmp) where
   mem m a := m.contains a
 
